src/3d/prelude/buffer/EverParse3d.Actions.All.fst
@@ -12,7 +12,7 @@ let ___PUINT8 = IB.puint8
 
 let action_field_ptr
       #nz #wk (#k:P.parser_kind nz wk) (#t:Type) (#p:P.parser k t) (u:unit)
-   = fun ctxt input startPosition _ ->
+   = fun ctxt _err input _len startPosition _ ->
        let open LowParse.Slice in
        IB.offset input.EverParse3d.InputStream.Buffer.Aux.buf (LowParse.Low.ErrorCode.uint64_to_uint32 startPosition) input.EverParse3d.InputStream.Buffer.Aux.perm_of
 
@@ -24,7 +24,7 @@ let action_field_ptr_after_with_setter _ = false_elim ()
 
 let action_field_pos_32
       #nz #wk (#k:P.parser_kind nz wk) (#t:Type) (#p:P.parser k t) (u:unit)
-   = fun ctxt input startPosition _ ->
+   = fun ctxt _err input _len startPosition _ ->
        [@inline_let]
        let res = LowParse.Low.ErrorCode.uint64_to_uint32 startPosition in
        assert (FStar.UInt32.v res == FStar.UInt64.v startPosition); // sanity-check: no modulo here
